src/impl/TLS13.Impl.Server.Driver.fsti
@@ -7,6 +7,8 @@ open Pulse.Lib.Array.PtsTo
 
 module B = TLS13.Bytes
 module Bounds = TLS13.Impl.ConnectionState.Bounds
+module CL = TLS13.ConnectionLog
+module CryptoSpec = TLS13.Crypto.Spec
 module CS = TLS13.Spec.ConnectionState
 module CM = TLS13.Impl.ConnectionState.Model
 module CR = TLS13.Impl.ConnectionState.Repr
@@ -15,6 +17,7 @@ module O = TLS13.OpenSSL
 module S = TLS13.Impl.Server
 module ST = TLS13.Impl.Server.Types
 module SZ = FStar.SizeT
+module T = TLS13.Types
 module U16 = FStar.UInt16
 module U8 = FStar.UInt8
 
@@ -188,3 +191,34 @@ fn generate_server_material_once
             'credential_identity
             'received
             'sent
+
+fn select_default_server_parameters_from_payload_once
+  (d:server_driver)
+  (payload:array U8.t)
+  (payload_len:SZ.t)
+  requires server_driver_connected
+              d
+              'st0
+              'certificate_chain
+              'credential_identity
+              'received
+              'sent **
+           pts_to payload 'payload_bytes **
+           pure (B.length 'payload_bytes == SZ.v payload_len /\
+                  SZ.v payload_len == 64 /\
+                  B.length (CL.raw_slice (Ghost.reveal 'payload_bytes) 0 32) == 32 /\
+                  B.length (CL.raw_slice (Ghost.reveal 'payload_bytes) 32 64) == 32 /\
+                  ST.server_local_event_input_ready
+                    'st0
+                    ST.LocalSelectServerParameters
+                    (Ghost.reveal 'payload_bytes))
+  returns resp:ST.server_response
+  ensures exists* st1.
+          server_driver_connected
+             d
+             st1
+             'certificate_chain
+             'credential_identity
+             'received
+             'sent **
+          pts_to payload 'payload_bytes
